simplified and corrected Hoare_Total.v

Hoare_Total.v
@@ -5,9 +5,9 @@ Definition hoaret_valid (P: assn) (c: com) (Q: assn): Prop :=
   forall s, P s -> (exists t, big_step (c, s) t /\ Q t ).
 
 Inductive hoaret: assn -> com -> assn -> Prop :=
-  | Skip  : forall P c, hoaret P c P
+  | Skip  : forall P, hoaret P Com.Skip P
   | Assign: forall P a x, hoaret (fun s => P (state_subst s a x)) (Com.Assign x a) P
-  | Seq   : forall P Q R c1 c2, hoaret P c1 Q -> hoare Q c2 R -> hoaret P (Com.Seq c1 c2) R
+  | Seq   : forall P Q R c1 c2, hoaret P c1 Q -> hoaret Q c2 R -> hoaret P (Com.Seq c1 c2) R
   | If    : forall P Q b c1 c2, hoaret (fun s => P s /\ bval s b = true)  c1 Q ->
                                   hoaret (fun s => P s /\ bval s b = false) c2 Q -> hoaret P (Com.If b c1 c2) Q
   | While : forall P b c (T: state -> nat -> Prop),
@@ -15,32 +15,34 @@ Inductive hoaret: assn -> com -> assn -> Prop :=
                  hoaret P (Com.While b c) (fun s => P s /\ bval s b = false)
   | conseq: forall (P P' Q Q': assn) c, (entails P' P) -> hoaret P c Q -> (entails Q Q') -> hoaret P' c Q'.
 
-Lemma While_fun: forall b (P Q: assn) c (f: state -> nat), 
-                   (forall n: nat, hoaret (fun s => P s /\ bval s b = true /\ n = f s) c (fun s => P s /\ f s < n)) ->
-                   hoaret P (Com.While b c) (fun s => P s /\ bval s b = false).
-Proof. intros.
+Lemma While_fun: forall b (P Q: assn) c (f: state -> nat),
+    (forall n: nat, hoaret (fun s => P s /\ bval s b = true /\ n = f s) c (fun s => P s /\ f s < n)) ->
+    hoaret P (Com.While b c) (fun s => P s /\ bval s b = false).
+Proof.
+       pose While; pose conseq; unfold entails in *; yelles 3.
+(*     intros.
        specialize (While P b c (fun s n => n = f s)); intros.
        apply H0. intros.
        eapply conseq.
        - Reconstr.scrush (** hammer *).
        - Reconstr.scrush (** hammer *).
-	     - Reconstr.hobvious Reconstr.Empty
-		     Reconstr.Empty
-		    (@Hoare.entails) (** hammer *).
+             - Reconstr.hobvious Reconstr.Empty
+                     Reconstr.Empty
+                    (@Hoare.entails) (** hammer *). *)
 Qed.
 
 Lemma strengthen_pre: forall (P P' Q: assn) c, (entails P' P) -> hoaret P c Q -> hoaret P' c Q.
 Proof.
-	Reconstr.hobvious Reconstr.Empty
-		(@conseq)
-		(@Hoare.entails) (** hammer *).
+        Reconstr.hobvious Reconstr.Empty
+                (@conseq)
+                (@Hoare.entails) (** hammer *).
 Qed.
 
 Lemma weaken_post: forall (P Q Q': assn) c, (entails Q Q') -> hoaret P c Q -> hoaret P c Q'.
 Proof.
-	Reconstr.hobvious Reconstr.Empty
-		(@conseq)
-		(@Hoare.entails) (** hammer *).
+        Reconstr.hobvious Reconstr.Empty
+                (@conseq)
+                (@Hoare.entails) (** hammer *).
 Qed.
 
 Lemma Assign': forall (P Q: assn) a x, (forall s, P s -> Q (state_subst s a x)) -> hoaret P (Com.Assign x a) Q.
@@ -49,22 +51,15 @@ Proof. intros.
        Reconstr.scrush (** hammer *).
 Qed.
 
-Lemma While_fun': forall b (P Q: assn) c (f: state -> nat), 
+Lemma While_fun': forall b (P Q: assn) c (f: state -> nat),
                  (forall n: nat, hoaret (fun s => P s /\ bval s b = true /\ n = f s) c (fun s => P s /\ f s < n)) ->
                  (forall s, P s /\ bval s b = false -> Q s) ->
                  hoaret P (Com.While b c) Q.
 Proof. intros.
-       specialize (While P b c (fun s n => n = f s)); intros.
-       specialize (weaken_post P (fun s : state => P s /\ bval s b = false) Q (Com.While b c)); intros.
-       apply H2.
-       Reconstr.scrush (** hammer *).
-       apply H1. intros.
-       eapply conseq.
-      - Reconstr.scrush (** hammer *).
-      - Reconstr.scrush (** hammer *).
-      - Reconstr.hobvious Reconstr.Empty
-		      Reconstr.Empty
-		      (@entails) (** hammer *).
+       apply (weaken_post P (fun s : state => P s /\ bval s b = false) Q (Com.While b c)).
+       - Reconstr.scrush (** hammer *).
+       - apply (While P b c (fun s n => n = f s)).
+         pose conseq; unfold entails in *; scrush.
 Qed.
 
 (** todos *)
@@ -72,14 +67,19 @@ Qed.
 (** prove soundness and completeness: this may take time..! *)
 
 Lemma hoaret_sound: forall P Q c, hoaret P c Q -> hoaret_valid P c Q.
-Proof. unfold hoare_valid. intros P Q c h.
-       induction h; try yelles 2.
+Proof.
+  unfold hoaret_valid; intros P Q c H.
+  induction H; intros s HH; sauto.
+  - Reconstr.hcrush Reconstr.AllHyps (@Big_Step.SeqSem) Reconstr.Empty.
+  - destruct (bval s b) eqn:?; pose Big_Step.IfTrue; pose Big_Step.IfFalse; scrush.
+  (* hammer finds a proof which cannot be reconstructed, because the
+     tactics can't guess that we need to destruct (bval s b); we do
+     this manually and use the dependencies found by CoqHammer *)
+  - assert (H1: forall n m s, m < n -> P s -> T s m ->
+                              exists t, (Com.While b c, s) ==> t /\ P t /\ bval t b = false).
+    induction n; intros.
+    destruct (bval s0 b) eqn:?; pose Big_Step.WhileFalse; scrush.
+    admit.
+    admit.
+  - scrush.
 Admitted.
-
-
-
-
-
-
-
-
